Add a name to struct and union types

ulib/FStar.Pointer.Base.fst
@@ -53,7 +53,7 @@ let step_typ_depth
 = match s with
   | StepUField l fd
   | StepField l fd ->
-    typ_depth_typ_of_struct_field l fd
+    typ_depth_typ_of_struct_field l.fields fd
   | _ -> ()
 
 let rec path_typ_depth
@@ -251,7 +251,7 @@ let rec dummy_val
       dummy_val (typ_of_struct_field l f)
     ))
   | TUnion l ->
-    let dummy_field : string = List.Tot.hd (List.Tot.map fst l) in
+    let dummy_field : string = List.Tot.hd (List.Tot.map fst l.fields) in
     union_create l dummy_field (dummy_val (typ_of_struct_field l dummy_field))
   | TArray length t -> Seq.create (UInt32.v length) (dummy_val t)
   | TPointer t -> Pointer t HS.dummy_aref PathBase
@@ -387,7 +387,7 @@ let struct_field_is_readable
   (v: ostruct l { Some? v } )
   (s: string)
 : Tot bool
-= if List.Tot.mem s (List.Tot.map fst l)
+= if List.Tot.mem s (List.Tot.map fst l.fields)
   then ovalue_is_readable (typ_of_struct_field l s) (ostruct_sel v s)
   else true
 
@@ -400,7 +400,7 @@ let rec ovalue_is_readable
   | TStruct l ->
     let (v: ostruct l) = v in
     Some? v && (
-      let keys = List.Tot.map fst l in
+      let keys = List.Tot.map fst l.fields in
       let pred
         (t': typ)
         (v: otype_of_typ t')
@@ -441,7 +441,7 @@ let ovalue_is_readable_struct_intro'
   (requires (
     let (v: ostruct l) = v in (
     Some? v /\
-    List.Tot.for_all (struct_field_is_readable l ovalue_is_readable v) (List.Tot.map fst l)
+    List.Tot.for_all (struct_field_is_readable l ovalue_is_readable v) (List.Tot.map fst l.fields)
   )))
   (ensures (ovalue_is_readable (TStruct l) v))
 = assert_norm (ovalue_is_readable (TStruct l) v == true)
@@ -457,7 +457,7 @@ let ovalue_is_readable_struct_intro
     ovalue_is_readable (typ_of_struct_field l f) (ostruct_sel v f)
   ))))
   (ensures (ovalue_is_readable (TStruct l) v))
-= List.Tot.for_all_mem (struct_field_is_readable l ovalue_is_readable v) (List.Tot.map fst l);
+= List.Tot.for_all_mem (struct_field_is_readable l ovalue_is_readable v) (List.Tot.map fst l.fields);
   ovalue_is_readable_struct_intro' l v
 
 let rec ovalue_is_readable_struct_elim
@@ -473,9 +473,9 @@ let rec ovalue_is_readable_struct_elim
   )))
   [SMTPat (ovalue_is_readable (typ_of_struct_field l fd) (ostruct_sel v fd))]
 = let (v: ostruct l) = v in
-  assert_norm (ovalue_is_readable (TStruct l) v == List.Tot.for_all (struct_field_is_readable l ovalue_is_readable v) (List.Tot.map fst l));
-  assert (List.Tot.for_all (struct_field_is_readable l ovalue_is_readable v) (List.Tot.map fst l));
-  List.Tot.for_all_mem (struct_field_is_readable l ovalue_is_readable v) (List.Tot.map fst l);
+  assert_norm (ovalue_is_readable (TStruct l) v == List.Tot.for_all (struct_field_is_readable l ovalue_is_readable v) (List.Tot.map fst l.fields));
+  assert (List.Tot.for_all (struct_field_is_readable l ovalue_is_readable v) (List.Tot.map fst l.fields));
+  List.Tot.for_all_mem (struct_field_is_readable l ovalue_is_readable v) (List.Tot.map fst l.fields);
   assert (ovalue_is_readable (typ_of_struct_field l fd) (ostruct_sel v fd))
 
 let ovalue_is_readable_array_elim
@@ -1249,7 +1249,10 @@ let path_includes_exists_concat
   (ensures (exists (r: path through to) . q == path_concat p r))
 = path_includes_ind
     (fun #to1_ #to2_ p1_ p2_ -> exists r . p2_ == path_concat p1_ r)
-    (fun #through #to_ p s -> FStar.Classical.exists_intro (fun r -> PathStep through to_ p s == path_concat p r) (PathStep through to_ PathBase s))
+    (fun #through #to_ p s -> 
+      let r = PathStep through to_ PathBase s in
+      assert_norm (PathStep through to_ p s == path_concat p r)
+    )
     (fun #to p -> FStar.Classical.exists_intro (fun r -> p == path_concat p r) PathBase)
     (fun #to1_ #to2_ #to3_ p1_ p2_ p3_ ->
       FStar.Classical.exists_elim  (exists r . p3_ == path_concat p1_ r) #_ #(fun r12 -> p2_ == path_concat p1_ r12) () (fun r12 ->
@@ -2369,7 +2372,7 @@ let readable_struct
   ))
   (ensures (readable h p))
 //  [SMTPat (readable #(TStruct l) h p)] // TODO: dubious pattern, will probably trigger unreplayable hints
-= let dummy_field : struct_field l = fst (List.Tot.hd l) in // struct is nonempty
+= let dummy_field : struct_field l = fst (List.Tot.hd l.fields) in // struct is nonempty
   let dummy_field_ptr = gfield p dummy_field in
   assert (readable h dummy_field_ptr);
   let content = greference_of p in
@@ -2412,7 +2415,7 @@ let rec readable_struct_fields'
   | [] -> True
   | f :: s' ->
     readable_struct_fields' h p s' /\ (
-      if List.Tot.mem f (List.Tot.map fst l)
+      if List.Tot.mem f (List.Tot.map fst l.fields)
       then
 	let f : struct_field l = f in
 	readable h (gfield p f)
@@ -2433,14 +2436,14 @@ let rec readable_struct_fields_elim
   (s: list string)
 : Lemma
   (requires (readable_struct_fields h p s))
-  (ensures (forall f . (List.Tot.mem f s /\ List.Tot.mem f (List.Tot.map fst l)) ==> (let f : struct_field l = f in readable h (gfield p f))))
+  (ensures (forall f . (List.Tot.mem f s /\ List.Tot.mem f (List.Tot.map fst l.fields)) ==> (let f : struct_field l = f in readable h (gfield p f))))
   (decreases s)
 = match s with
   | [] -> ()
   | _ :: q -> readable_struct_fields_elim h p q
 
 let readable_struct_fields_readable_struct #l h p =
-  readable_struct_fields_elim h p (List.Tot.map fst l);
+  readable_struct_fields_elim h p (List.Tot.map fst l.fields);
   readable_struct h p
 
 let readable_gcell
@@ -3425,6 +3428,8 @@ let rec loc_aux_syntactically_includes_trans
       (fun _ -> loc_aux_syntactically_includes_trans sl s2 s3)
       (fun _ -> loc_aux_syntactically_includes_trans sr s2 s3)
   | _ -> ()
+
+#set-options "--initial_fuel 2 --max_fuel 2"
 
 let loc_aux_syntactically_includes_union_r
   (s1 s2 s3: loc_aux)
